Splitting lucas in pieces

num/Lucas.v
@@ -75,12 +75,92 @@ Let square_m2 :=
    let sub := m_op.(sub_mod) in
    fun x => sub (square x) w2.
 
-Definition lucastest :=
- ZnZ.to_Z (iter_pos _ square_m2 w4 (Pminus p 2)).
+Definition lucastest_step x p := iter_pos _ square_m2 x p.
 
-Theorem lucastest_aux_correct:
+Lemma square_m2_bounded x : 0 <= [|x|] < [|b|] -> 0 <= [|square_m2 x|] < [|b|].
+Proof.
+intro H.
+unfold square_m2.
+rewrite (sub_mod_spec m_op_spec _ _  [|square_mod m_op x|] 2).
+apply Z.mod_pos_bound; auto with zarith.
+rewrite Z.mod_small; auto with zarith.
+rewrite (square_mod_spec m_op_spec x [|x|]); auto.
+apply Z.mod_pos_bound; auto with zarith.
+rewrite Z.mod_small; auto with zarith.
+exact w2_b.
+Qed.
+
+Lemma lucastest_bounded x p1 : 0 <= [|x|] < [|b|] ->
+  0 <= [|lucastest_step x p1|] < [|b|].
+Proof.
+unfold lucastest_step.
+revert p1 x.
+intros p1; pattern p1; apply Pind; simpl iter_pos; simpl s; clear p1.
+exact square_m2_bounded.
+intros p1 IH x Hx.
+rewrite Pos.iter_succ.
+apply square_m2_bounded.
+apply IH; auto.
+Qed.
+
+Lemma square_m2_eq x1 x2 :
+ [|x1|] < [|b|] ->
+[|x1|] = [|x2|] -> [|square_m2 x1|] = [|square_m2 x2|].
+Proof.
+intros Hx1 Ex1.
+assert (H1 : [|x1|] = [|x1|] mod [|b|]).
+rewrite Z.mod_small; auto with zarith.
+case (ZnZ.spec_to_Z x1); auto with zarith.
+assert (H2 : [|x2|] = [|x2|] mod [|b|]).
+rewrite <- Ex1; auto.
+unfold square_m2.
+rewrite (sub_mod_spec m_op_spec _ _  [|square_mod m_op x1|] 2).
+rewrite (sub_mod_spec m_op_spec _ _  [|square_mod m_op x2|] 2).
+rewrite (square_mod_spec m_op_spec x1 [|x1|]); auto.
+rewrite (square_mod_spec m_op_spec x2 [|x2|]); auto.
+rewrite Ex1; auto.
+rewrite Z.mod_small; auto with zarith.
+rewrite (square_mod_spec m_op_spec x2 [|x2|]); auto.
+apply Z.mod_bound_pos; auto with zarith.
+apply Z.square_nonneg.
+exact w2_b.
+rewrite Z.mod_small; auto with zarith.
+rewrite (square_mod_spec m_op_spec x1 [|x1|]); auto.
+apply Z.mod_bound_pos; auto with zarith.
+apply Z.square_nonneg.
+exact w2_b.
+Qed.
+
+Lemma lucastest_eq x1 x2 p1 : [|x1|] < [|b|] ->
+  [|x1|] = [|x2|] -> [|lucastest_step x1 p1|] =  [|lucastest_step x2 p1|].
+Proof.
+unfold lucastest_step.
+revert p1 x1 x2.
+intros p1; pattern p1; apply Pind; simpl iter_pos; simpl s; clear p1.
+exact square_m2_eq.
+intros p1 IH x1 x2 Hx1 Hx2.
+rewrite !Pos.iter_succ.
+apply square_m2_eq.
+assert (F : 0 <= [|x1|] < [|b|]).
+case (ZnZ.spec_to_Z x1); auto with zarith.
+generalize (lucastest_bounded _ p1 F).
+unfold lucastest_step; auto with zarith.
+apply IH; auto.
+Qed.
+
+Theorem lucastest_step_add :
+ forall p1 p2 z z1 z2, lucastest_step z p1 = z1 ->
+        lucastest_step z1 p2 = z2 -> lucastest_step z (p2 + p1) = z2.
+Proof.
+unfold lucastest_step.
+intros p1 p2 z z1 z2 H1 H2.
+rewrite Pos.iter_add, H1; auto.
+Qed.
+
+Theorem lucastest_step_correct:
  forall p1 z n, 0 <= n -> [|z|] = fst (s n) mod (2 ^ Zpos p - 1) ->
-       [|iter_pos _ square_m2 z p1|] = fst (s (n + Zpos p1)) mod (2 ^ Zpos p - 1).
+       [|lucastest_step z p1|] = fst (s (n + Zpos p1)) mod (2 ^ Zpos p - 1).
+unfold lucastest_step.
 intros p1; pattern p1; apply Pind; simpl iter_pos; simpl s; clear p1.
 intros z p1 Hp1 H.
 unfold square_m2.
@@ -110,10 +190,12 @@ rewrite sn; simpl fst; try rewrite b_p; auto with zarith.
 rewrite Zpos_plus_distr; auto with zarith.
 Qed.
 
+Definition lucastest := [|lucastest_step w4 (Pminus p 2)|].
+
 Theorem lucastest_prop: lucastest = fst(s (Zpos p -2)) mod (2 ^ Zpos p - 1).
 unfold lucastest.
 assert (F: 0 <= 0); auto with zarith.
-generalize (lucastest_aux_correct (p -2) w4 F); simpl Zplus;
+generalize (lucastest_step_correct (p -2) w4 F); simpl Zplus;
    rewrite Zpos_minus; auto with zarith.
 rewrite Zmax_right; auto with zarith.
 intros tmp; apply tmp; clear tmp.
@@ -167,22 +249,28 @@ Definition lucas p :=
  let mod_op := mmake_mod_op op b zp in
   lucastest op p mod_op.
 
-Theorem lucas_prime:
- forall p, 2 < Zpos p -> lucas p = 0 -> prime (2 ^ Zpos p - 1).
-unfold lucas; intros p Hp H.
-match type of H with lucastest (cmk_op ?x) ?y ?z = _ =>
-   set (w_op := (cmk_op x)); assert(A1: ZnZ.Specs w_op)
-end.
-unfold w_op; apply cmk_spec.
-assert (F0: Zpos p <= Zpos (ZnZ.digits w_op)).
-unfold w_op, base; rewrite (cmk_op_digits (Peano.pred (nat_of_P (get_height 31 p)))).
+Section LucasStep.
+
+Let op p  := cmk_op (Peano.pred (nat_of_P (get_height 31 p))).
+Let b p := znz_of_Z (op p) (2 ^ (Zpos p) - 1).
+Let zp p := znz_of_Z (op p) (Zpos p).
+Let mod_op p := mmake_mod_op (op p) (b p) (zp p).
+
+Let lucas_f1 p : (2 < p)%positive -> Zpos p <= Zpos (ZnZ.digits (op p)).
+Proof.
+intros Hp.
+unfold op, base; rewrite cmk_op_digits.
 generalize (get_height_correct 31 p).
 replace (Z_of_nat (Peano.pred (nat_of_P (get_height 31 p)))) with
        ((Zpos (get_height 31 p) - 1) ); auto with zarith.
 rewrite pred_of_minus; rewrite inj_minus1; auto with zarith.
 rewrite <- Zpos_eq_Z_of_nat_o_nat_of_P; auto with zarith.
 generalize (lt_O_nat_of_P (get_height 31 p)); auto with zarith.
-assert (F1: ZnZ.to_Z (znz_of_Z w_op (2 ^ (Zpos p) - 1)) = 2 ^ (Zpos p) - 1).
+Qed.
+
+Let lucas_f2 p : (2 < p)%positive -> @ZnZ.to_Z _ (op p) (b p) = 2 ^ (Zpos p) - 1.
+Proof.
+unfold b; intros Hp.
 assert (F1: 0 < 2 ^ (Zpos p) - 1).
 assert (F2: 2 ^ 0 < 2 ^ (Zpos p)); auto with zarith.
 apply Zpower_lt_monotone; auto with zarith.
@@ -191,23 +279,165 @@ case_eq (2 ^ (Zpos p) - 1); simpl ZnZ.to_Z.
 intros HH; contradict F1; rewrite HH; auto with zarith.
 2: intros p1 HH; contradict F1; rewrite HH; 
   apply Zle_not_lt; red; simpl; intros; discriminate.
-intros p1 Hp1; apply ZnZ.of_pos_correct; auto.
+intros p1 Hp1; apply (@ZnZ.of_pos_correct _ (op p)); auto.
+apply cmk_spec.
 rewrite <- Hp1.
 unfold base.
 apply Zlt_le_trans with (2 ^ (Zpos p)); auto with zarith.
 apply Zpower_le_monotone; auto with zarith.
-match type of H with lucastest (cmk_op ?x) ?y ?z = _ =>
-  apply  
-  (@lucastest_prime _ _ (cmk_spec x) p (znz_of_Z w_op (2 ^ Zpos p  -1)) Hp F1 z)
-end; auto with zarith; fold w_op.
-eapply mmake_mod_spec with (p := p); auto with zarith.
-unfold znz_of_Z; unfold znz_of_Z in F1; rewrite F1.
+Qed.
+
+Let lucas_f3 p :(2 < p)%positive -> mod_spec (op p) (b p) (mod_op p).
+Proof.
+intro Hp.
+assert (F1 : ZnZ.Specs (op p)).
+  apply cmk_spec; auto.
+apply mmake_mod_spec with (p := p); auto.
+rewrite lucas_f2; auto.
 assert (F2: 2 ^ 1 < 2 ^ (Zpos p)); auto with zarith.
 apply Zpower_lt_monotone; auto with zarith.
+assert (2 < Z.pos p); auto with zarith.
 rewrite Zpower_1_r in F2; auto with zarith.
-rewrite ZnZ.of_Z_correct; auto with zarith.
+unfold zp.
+apply ZnZ.of_Z_correct.
 split; auto with zarith.
-apply Zle_lt_trans with (1 := F0); auto with zarith.
+apply Zle_lt_trans with (1 := lucas_f1 Hp); auto with zarith.
 unfold base; apply Zpower2_lt_lin; auto with zarith.
 Qed.
+
+Theorem lucas_prime:
+ forall p, 2 < Zpos p -> lucas p = 0 -> prime (2 ^ Zpos p - 1).
+intros p Hp H.
+assert(A1: ZnZ.Specs (op p)).
+apply cmk_spec; auto.
+apply (lucastest_prime A1 Hp (lucas_f2 Hp) (lucas_f3 Hp) H).
+Qed.
+
+Definition lucas_step p x p1 :=
+ let op := cmk_op (Peano.pred (nat_of_P (get_height 31 p))) in
+ let b := znz_of_Z op (Zpower 2 (Zpos p) - 1) in
+ let zp := znz_of_Z op (Zpos p) in
+ let mod_op := mmake_mod_op op b zp in
+  ZnZ.to_Z (lucastest_step op mod_op (znz_of_Z op x) p1).
+
+Lemma lucasE p : 2 < Zpos p -> lucas_step p 4 (p - 2) = 0 -> lucas p = 0.
+Proof.
+intros H.
+unfold lucas, lucas_step, lucastest.
+set (o := cmk_op _).
+set (m := mmake_mod_op _ _ _).
+assert (F0 : 1 < ZnZ.to_Z (b p)).
+replace (ZnZ.to_Z (b p)) with (2 ^ Z.pos p - 1); auto with zarith.
+assert (2 ^ 1 <  2 ^ Z.pos p); auto with zarith.
+apply Zpower_lt_monotone; auto with zarith.
+replace (2 ^ 1) with 2 in H0; auto with zarith.
+rewrite <-(lucas_f2 H); auto.
+assert (F1 : ZnZ.to_Z ZnZ.one = 1).
+rewrite w1_b with (p := p) (b := b p); auto.
+rewrite Z.mod_small; auto with zarith.
+apply cmk_spec; auto.
+rewrite <-(lucas_f2 H); auto.
+assert (F2 : ZnZ.to_Z ZnZ.one = 1 mod ZnZ.to_Z (b p)).
+rewrite Z.mod_small; auto with zarith.
+intro H1; rewrite <-H1.
+assert (F3 : ZnZ.to_Z (add_mod m ZnZ.one ZnZ.one) = 2 mod ZnZ.to_Z (b p)).
+rewrite (add_mod_spec (lucas_f3 H) _ _ 1 1); auto.
+replace (ZnZ.to_Z ZnZ.one) with 1; auto.
+apply lucastest_eq with (p := p) (b := b p); auto.
+apply cmk_spec; auto.
+apply lucas_f2; auto.
+apply lucas_f3; auto.
+rewrite (add_mod_spec (lucas_f3 H) _ _ 2 2); auto.
+match goal with |- ?X < ?Y => assert (0 <= X < Y) end; auto with zarith.
+apply Z.mod_pos_bound; auto with zarith.
+rewrite (add_mod_spec (lucas_f3 H) _ _ 2 2); auto.
+replace ((ZnZ.to_Z (add_mod m ZnZ.one ZnZ.one))) with (2 mod ZnZ.to_Z (b p)).
+rewrite <-Z.add_mod; auto with zarith.
+rewrite Z.mod_small.
+simpl.
+apply sym_equal.
+apply (@ZnZ.of_pos_correct _ o).
+apply cmk_spec; auto.
+replace 4 with (2 ^ 2); auto with zarith.
+apply Zpower_lt_monotone; auto with zarith.
+split; auto with zarith.
+assert (F := lucas_f1 H); auto with zarith.
+unfold op in F; simpl in F; unfold o; auto with zarith.
+split; auto with zarith.
+replace (2 + 2) with (2 ^ 2); auto with zarith.
+replace (ZnZ.to_Z (b p)) with (2 ^ Z.pos p - 1); auto with zarith.
+assert (2 ^ 3 <=  2 ^ Z.pos p); auto with zarith.
+apply Zpower_le_monotone; auto with zarith.
+replace (2 ^ 3) with 8 in H0; auto with zarith.
+replace (2 ^ 2) with 4; auto with zarith.
+rewrite <-(lucas_f2 H); auto.
+generalize F0.
+auto with zarith.
+set (u := ZnZ.to_Z _).
+auto with zarith.
+Qed.
+
+Theorem lucas_step_add p p1 p2 z z1 z2 :
+   (2 < Zpos p) -> 0 <= z < 2 ^ (Zpos p) - 1 ->
+   lucas_step p z p1 = z1 -> lucas_step  p z1 p2 = z2 -> lucas_step p z (p2 + p1) = z2.
+Proof.
+intros H H0 H1 H2.
+assert(A1: ZnZ.Specs (op p)).
+apply cmk_spec; auto.
+unfold lucas_step.
+set (o := cmk_op _).
+set (m := mmake_mod_op _ _ _).
+assert (F1 : forall z3, 0 <= z3 < ZnZ.to_Z (b p) -> ZnZ.to_Z (znz_of_Z o z3) = z3).
+intro z3.
+case z3; simpl; auto with zarith.
+rewrite ZnZ.spec_0; auto.
+intros p3 [H3 H4].
+apply ZnZ.of_pos_correct.
+apply Zlt_le_trans with (1 := H4).
+replace (ZnZ.to_Z (b p)) with (2 ^ Z.pos p - 1).
+assert (2 ^ Zpos p <= base (ZnZ.digits o)); auto with zarith.
+apply Zpower_le_monotone; auto with zarith.
+assert (F := lucas_f1 H); auto with zarith.
+rewrite <-(lucas_f2 H); auto.
+intros p3 []; unfold Zle; simpl; intros H3; case H3; auto.
+unfold lucastest_step.
+rewrite Pos.iter_add; auto. 
+change (@ZnZ.to_Z _ o (lucastest_step o m (lucastest_step o m (znz_of_Z o z) p1) p2) = z2).
+assert (F :  ZnZ.to_Z (lucastest_step  o m (znz_of_Z o z) p1) = 
+            ZnZ.to_Z (znz_of_Z o z1)).
+unfold lucas_step in H1; fold o in H1; fold m in H1; rewrite H1.
+rewrite F1; auto.
+rewrite <- H1.
+apply (lucastest_bounded A1 H (lucas_f2 H) (lucas_f3 H)).
+rewrite F1.
+rewrite (lucas_f2 H); auto with zarith.
+replace (ZnZ.to_Z (b p)) with (2 ^ Z.pos p - 1); auto with zarith.
+rewrite <-(lucas_f2 H); auto with zarith.
+rewrite lucastest_eq with (p := p) (b := b p) (6 := F); auto.
+apply lucas_f2; auto.
+apply lucas_f3; auto.
+assert (0 <=  ZnZ.to_Z (lucastest_step o m (znz_of_Z o z) p1) < ZnZ.to_Z (b p)).
+apply (lucastest_bounded A1 H (lucas_f2 H) (lucas_f3 H)).
+rewrite F1.
+replace (ZnZ.to_Z (b p)) with (2 ^ Z.pos p - 1); auto with zarith.
+rewrite <-(lucas_f2 H); auto with zarith.
+replace (ZnZ.to_Z (b p)) with (2 ^ Z.pos p - 1); auto with zarith.
+rewrite <-(lucas_f2 H); auto with zarith.
+auto with zarith.
+Qed.
+
+Lemma lucas_step_same_p : forall p x p1 p2 z,
+   p1 = p2 -> lucas_step p x p1 = z -> lucas_step p x p2 = z.
+Proof.
+intros p x p1 p2 z Hp Hz.
+apply trans_equal with (2 := Hz).
+apply f_equal2 with (f := lucas_step p); auto.
+Qed.
+
+End LucasStep.
+
+Ltac vmtac :=
+match goal with |- _ = ?x =>
+vm_cast_no_check  (refl_equal x)
+end.
 
